Finished depth-threading

06TailCall/TailCall.thy
@@ -3,8 +3,8 @@ theory TailCall
 begin
 
 datatype tco_return =
-    TCOReturn
-  | TCOJump
+    TCOReturn nat
+  | TCOJump nat
 
 datatype tco_code = 
   TCOLookup nat
@@ -29,9 +29,10 @@ inductive evaltco :: "tco_code_state \<Rightarrow> tco_code_state \<Rightarrow> 
     TCOS (TCOLam env cd' r' # vs) ((env, cd, r) # sfs)"
 | evtco_apply [simp]: "TCOS (v # TCOLam env' cd' r' # vs) ((env, TCOApply # cd, r) # sfs) \<leadsto>\<^sub>t\<^sub>c\<^sub>o 
     TCOS vs ((v # env', cd', r') # (env, cd, r) # sfs)"
-| evtco_return [simp]: "TCOS vs ((env, [], TCOReturn) # sfs) \<leadsto>\<^sub>t\<^sub>c\<^sub>o TCOS vs sfs"
-| evtco_jump [simp]: "TCOS (v # TCOLam env' cd' r' # vs) ((env, [], TCOJump) # sfs) \<leadsto>\<^sub>t\<^sub>c\<^sub>o 
-    TCOS vs ((v # env', cd', r') # sfs)"
+| evtco_return [simp]: "TCOS vs ((env, [], TCOReturn (length env)) # sfs) \<leadsto>\<^sub>t\<^sub>c\<^sub>o TCOS vs sfs"
+| evtco_jump [simp]: 
+    "TCOS (v # TCOLam env' cd' r' # vs) ((env, [], TCOJump (length env)) # sfs) \<leadsto>\<^sub>t\<^sub>c\<^sub>o 
+      TCOS vs ((v # env', cd', r') # sfs)"
 
 theorem determinismt: "\<Sigma> \<leadsto>\<^sub>t\<^sub>c\<^sub>o \<Sigma>' \<Longrightarrow> \<Sigma> \<leadsto>\<^sub>t\<^sub>c\<^sub>o \<Sigma>'' \<Longrightarrow> \<Sigma>' = \<Sigma>''"
 proof (induction \<Sigma> \<Sigma>' rule: evaltco.induct)
@@ -56,11 +57,13 @@ next
        simp_all 
 next
   case (evtco_return vs env sfs)
-  thus ?case by (induction "TCOS vs ((env, [], TCOReturn) # sfs)" \<Sigma>'' rule: evaltco.induct) simp_all 
+  thus ?case 
+    by (induction "TCOS vs ((env, [], TCOReturn (length env)) # sfs)" \<Sigma>'' rule: evaltco.induct)
+       simp_all 
 next
   case (evtco_jump v env' cd' r' vs env sfs)
   thus ?case 
-    by (induction "TCOS (v # TCOLam env' cd' r' # vs) ((env, [], TCOJump) # sfs)" \<Sigma>''
+    by (induction "TCOS (v # TCOLam env' cd' r' # vs) ((env, [], TCOJump (length env)) # sfs)" \<Sigma>''
         rule: evaltco.induct) 
        simp_all 
 qed
