06TailCall/TailCallOptimization.thy
@@ -2,34 +2,34 @@ theory TailCallOptimization
   imports TailCall "../05TreeCode/TreeCode" "../00Utils/Iteration"
 begin
 
-fun tco_r :: "tree_code list \<Rightarrow> tco_return" where
-  "tco_r [] = TCOReturn"
-| "tco_r (TApply # cd) = (case cd of 
-      [] \<Rightarrow> TCOJump
-    | _ \<Rightarrow> tco_r cd)"
-| "tco_r (op # cd) = tco_r cd"
+fun tco_r :: "nat \<Rightarrow> tree_code list \<Rightarrow> tco_return" where
+  "tco_r d [] = TCOReturn d"
+| "tco_r d (TApply # cd) = (case cd of 
+      [] \<Rightarrow> TCOJump d
+    | _ \<Rightarrow> tco_r d cd)"
+| "tco_r d (op # cd) = tco_r d cd"
 
 fun tco_cd :: "tree_code list \<Rightarrow> tco_code list" where
   "tco_cd [] = []"
 | "tco_cd (TLookup x # cd) = TCOLookup x # tco_cd cd"
 | "tco_cd (TPushCon k # cd) = TCOPushCon k # tco_cd cd"
-| "tco_cd (TPushLam cd' d # cd) = TCOPushLam (tco_cd cd') (tco_r cd') d # tco_cd cd"
+| "tco_cd (TPushLam cd' d # cd) = TCOPushLam (tco_cd cd') (tco_r (Suc d) cd') d # tco_cd cd"
 | "tco_cd (TApply # cd) = (case cd of 
       [] \<Rightarrow> []
     | _ \<Rightarrow> TCOApply # tco_cd cd)"
 
 definition tco :: "tree_code list \<Rightarrow> tco_code list \<times> tco_return" where
-  "tco cd = (tco_cd cd, tco_r cd)"
+  "tco cd = (tco_cd cd, tco_r 0 cd)"
 
 primrec tco_val :: "tclosure \<Rightarrow> tco_closure" where
   "tco_val (TConst k) = TCOConst k"
-| "tco_val (TLam vs cd) = TCOLam (map tco_val vs) (tco_cd cd) (tco_r cd)"
+| "tco_val (TLam vs cd) = TCOLam (map tco_val vs) (tco_cd cd) (tco_r (Suc (length vs)) cd)"
 
 fun tco_stack_frame :: "tree_stack_frame \<Rightarrow> tco_stack_frame" where
-  "tco_stack_frame (vs, cd) = (map tco_val vs, tco_cd cd, tco_r cd)"
+  "tco_stack_frame (vs, cd) = (map tco_val vs, tco_cd cd, tco_r (length vs) cd)"
 
 fun not_dead_frame :: "tco_stack_frame \<Rightarrow> bool" where
-  "not_dead_frame (vs, cd, r) = (cd \<noteq> [] \<or> r \<noteq> TCOReturn)"
+  "not_dead_frame (vs, cd, r) = (cd \<noteq> [] \<or> r \<noteq> TCOReturn (length vs))"
 
 primrec dead_frame :: "tree_stack_frame \<Rightarrow> bool" where
   "dead_frame (vs, cd) = (cd = [])"
@@ -41,8 +41,8 @@ primrec tco_state :: "tree_code_state \<Rightarrow> tco_code_state" where
   "tco_state (TS vs sfs) = TCOS (map tco_val vs) (tco_stack sfs)"
 
 lemma [dest]: "(env, cd, r) # sfs = tco_stack sfs' \<Longrightarrow> \<exists>dsfs env' cd' sfs''. 
-  sfs' = dsfs @ (env', cd') # sfs'' \<and> env = map tco_val env' \<and> cd = tco_cd cd' \<and> r = tco_r cd' \<and> 
-    list_all dead_frame dsfs \<and> sfs = tco_stack sfs''"
+  sfs' = dsfs @ (env', cd') # sfs'' \<and> env = map tco_val env' \<and> cd = tco_cd cd' \<and> 
+    r = tco_r (length env) cd' \<and> list_all dead_frame dsfs \<and> sfs = tco_stack sfs''"
 proof (induction sfs')
   case (Cons sf sfs')
   thus ?case
@@ -52,8 +52,8 @@ proof (induction sfs')
     proof (induction cd' rule: tco_cd.induct)
       case 1
       then obtain dsfs env'' cd' sfs'' where X: "sfs' = dsfs @ (env'', cd') # sfs'' \<and> 
-        env = map tco_val env'' \<and> cd = tco_cd cd' \<and> r = tco_r cd' \<and> list_all dead_frame dsfs \<and> 
-          sfs = tco_stack sfs''" by auto
+        env = map tco_val env'' \<and> cd = tco_cd cd' \<and> r = tco_r (length env'') cd' \<and> 
+          list_all dead_frame dsfs \<and> sfs = tco_stack sfs''" by auto
       hence "\<exists>dsfsx. (env', []) # dsfs @ (env'', cd') # sfs'' = dsfsx @ (env'', cd') # sfs'' \<and> 
           list_all dead_frame dsfsx \<and> sfs = tco_stack sfs''" by simp
       hence "\<exists>dsfsx sfs'''. 
@@ -62,31 +62,32 @@ proof (induction sfs')
       with X show ?case by fastforce
     next
       case (2 x cd')
-      hence "env = map tco_val env' \<and> cd = TCOLookup x # tco_cd cd' \<and> r = tco_r cd' \<and> 
+      hence "env = map tco_val env' \<and> cd = TCOLookup x # tco_cd cd' \<and> r = tco_r (length env') cd' \<and> 
         sfs = tco_stack sfs'" by simp
       thus ?case by fastforce
     next
       case (3 k cd')
-      hence "env = map tco_val env' \<and> cd = TCOPushCon k # tco_cd cd' \<and> r = tco_r cd' \<and> 
-        sfs = tco_stack sfs'" by simp
+      hence "env = map tco_val env' \<and> cd = TCOPushCon k # tco_cd cd' \<and> 
+        r = tco_r (length env') cd' \<and> sfs = tco_stack sfs'" by simp
       thus ?case by fastforce
     next
       case (4 cd\<^sub>l d cd')
-      hence "env = map tco_val env' \<and> cd = TCOPushLam (tco_cd cd\<^sub>l) (tco_r cd\<^sub>l) d # tco_cd cd' \<and> 
-        r = tco_r cd' \<and> sfs = tco_stack sfs'" by simp
+      hence "env = map tco_val env' \<and> 
+        cd = TCOPushLam (tco_cd cd\<^sub>l) (tco_r (Suc d) cd\<^sub>l) d # tco_cd cd' \<and> 
+          r = tco_r (length env') cd' \<and> sfs = tco_stack sfs'" by simp
       thus ?case by fastforce
     next
       case (5 cd')
       thus ?case
       proof (cases cd')
         case Nil
-        moreover with 5 have "env = map tco_val env' \<and> cd = [] \<and> r = TCOJump \<and> 
+        moreover with 5 have "env = map tco_val env' \<and> cd = [] \<and> r = TCOJump (length env') \<and> 
           sfs = tco_stack sfs'" by simp
         ultimately show ?thesis by fastforce
       next
         case (Cons op cd'')
         moreover with 5 have "env = map tco_val env' \<and> cd = TCOApply # tco_cd (op # cd'') \<and> 
-          r = tco_r (op # cd'') \<and> sfs = tco_stack sfs'" by simp
+          r = tco_r (length env') (op # cd'') \<and> sfs = tco_stack sfs'" by simp
         ultimately show ?thesis by fastforce
       qed
     qed
@@ -95,7 +96,7 @@ qed simp_all
 
 lemma [dest]: "TCOS vs ((env, cd, r) # sfs) = tco_state \<Sigma> \<Longrightarrow> \<exists>dsfs vs' env' cd' sfs'. 
   \<Sigma> = TS vs' (dsfs @ (env', cd') # sfs') \<and> vs = map tco_val vs' \<and> env = map tco_val env' \<and> 
-    cd = tco_cd cd' \<and> r = tco_r cd' \<and> list_all dead_frame dsfs \<and> sfs = tco_stack sfs'"
+    cd = tco_cd cd' \<and> r = tco_r (length env) cd' \<and> list_all dead_frame dsfs \<and> sfs = tco_stack sfs'"
   by (induction \<Sigma>) auto
 
 lemma [dest]: "TCOLookup x # cd = tco_cd cd' \<Longrightarrow> \<exists>cd''. cd' = TLookup x # cd'' \<and> cd = tco_cd cd''"
@@ -110,16 +111,16 @@ proof (induction dsfs)
 qed simp_all
 
 lemma [simp]: "\<exists>\<Sigma>\<^sub>t \<Sigma>. iter (\<leadsto>\<^sub>t) (TS vs ((env, cd) # sfs)) \<Sigma>\<^sub>t \<and> 
-  iter (\<leadsto>\<^sub>t\<^sub>c\<^sub>o) (TCOS (map tco_val vs) ((map tco_val env, tco_cd cd, tco_r cd) # tco_stack sfs)) \<Sigma> \<and> 
-    \<Sigma> = tco_state \<Sigma>\<^sub>t" 
+  iter (\<leadsto>\<^sub>t\<^sub>c\<^sub>o) (TCOS (map tco_val vs) 
+    ((map tco_val env, tco_cd cd, tco_r (length env) cd) # tco_stack sfs)) \<Sigma> \<and> \<Sigma> = tco_state \<Sigma>\<^sub>t" 
 proof (induction cd rule: tco_cd.induct)
   case 1
   have "TS vs ((env, []) # sfs) \<leadsto>\<^sub>t TS vs sfs" by simp
   hence X: "iter (\<leadsto>\<^sub>t) (TS vs ((env, []) # sfs)) (TS vs sfs)" by (metis iter_one)
-  have "TCOS (map tco_val vs) ((map tco_val env, tco_cd [], tco_r []) # tco_stack sfs) \<leadsto>\<^sub>t\<^sub>c\<^sub>o
-    TCOS (map tco_val vs) (tco_stack sfs)" by simp
+  have "TCOS (map tco_val vs) ((map tco_val env, tco_cd [], tco_r (length env) []) # tco_stack sfs) 
+    \<leadsto>\<^sub>t\<^sub>c\<^sub>o TCOS (map tco_val vs) (tco_stack sfs)" by simp
   hence Y: "iter (\<leadsto>\<^sub>t\<^sub>c\<^sub>o) 
-    (TCOS (map tco_val vs) ((map tco_val env, tco_cd [], tco_r []) # tco_stack sfs)) 
+    (TCOS (map tco_val vs) ((map tco_val env, tco_cd [], tco_r (length env) []) # tco_stack sfs)) 
       (TCOS (map tco_val vs) (tco_stack sfs))" by (metis iter_one)
   have "TCOS (map tco_val vs) (tco_stack sfs) = tco_state (TS vs sfs)" by simp
   with X Y show ?case by blast
@@ -148,8 +149,8 @@ theorem completetco [simp]: "tco_state \<Sigma>\<^sub>t \<leadsto>\<^sub>t\<^sub
 proof (induction "tco_state \<Sigma>\<^sub>t" \<Sigma>' rule: evaltco.induct)
   case (evtco_lookup env x v vs cd r sfs)
   then obtain dsfs vs' env' cd' sfs' where S: "\<Sigma>\<^sub>t = TS vs' (dsfs @ (env', cd') # sfs') \<and> 
-    vs = map tco_val vs' \<and> env = map tco_val env' \<and> TCOLookup x # cd = tco_cd cd' \<and> r = tco_r cd' \<and> 
-      list_all dead_frame dsfs \<and> sfs = tco_stack sfs'" by blast
+    vs = map tco_val vs' \<and> env = map tco_val env' \<and> TCOLookup x # cd = tco_cd cd' \<and> 
+      r = tco_r (length env) cd' \<and> list_all dead_frame dsfs \<and> sfs = tco_stack sfs'" by blastx
   then obtain cd'' where C: "cd' = TLookup x # cd'' \<and> cd = tco_cd cd''" by blast
   from evtco_lookup S obtain v' where V: "lookup env' x = Some v' \<and> v = tco_val v'" by auto
   hence "TS vs' ((env', TLookup x # cd'') # sfs') \<leadsto>\<^sub>t TS (v' # vs') ((env', cd'') # sfs')" by simp
@@ -179,10 +180,10 @@ next
   then show ?case by simp
 qed
 
-lemma [simp]: "tco_cd (op # cd) = [] \<Longrightarrow> tco_r (op # cd) = TCOJump"
+lemma [simp]: "tco_cd (op # cd) = [] \<Longrightarrow> tco_r d (op # cd) = TCOJump d"
   by (induction op) (simp_all split: list.splits)
 
-lemma tco_never_dead [simp]: "not_dead_frame (vs, tco_cd (op # cd), tco_r (op # cd))"
+lemma tco_never_dead [simp]: "not_dead_frame (vs, tco_cd (op # cd), tco_r (length vs) (op # cd))"
   by (induction cd rule: tco_cd.induct) (simp_all split: list.splits)
 
 theorem correcttco [simp]: "\<Sigma> \<leadsto>\<^sub>t \<Sigma>' \<Longrightarrow> iter (\<leadsto>\<^sub>t\<^sub>c\<^sub>o) (tco_state \<Sigma>) (tco_state \<Sigma>')"
@@ -191,11 +192,15 @@ proof (induction \<Sigma> \<Sigma>' rule: evalt.induct)
   thus ?case 
   proof (cases cd)
     case Nil
-    from evt_lookup have "tco_state (TS vs ((env, [TLookup x]) # sfs)) \<leadsto>\<^sub>t\<^sub>c\<^sub>o
-      TCOS (tco_val v # map tco_val vs) ((map tco_val env, [], TCOReturn) # tco_stack sfs)" by simp
-    moreover have "TCOS (tco_val v # map tco_val vs) 
-      ((map tco_val env, [], TCOReturn) # tco_stack sfs) \<leadsto>\<^sub>t\<^sub>c\<^sub>o 
+    have "TCOS (tco_val v # map tco_val vs) 
+      ((map tco_val env, [], TCOReturn (length env)) # tco_stack sfs) \<leadsto>\<^sub>t\<^sub>c\<^sub>o 
+        TCOS (tco_val v # map tco_val vs) (tco_stack sfs)" by (metis evtco_return length_map)
+    hence "TCOS (tco_val v # map tco_val vs) 
+      ((map tco_val env, [], TCOReturn (length env)) # tco_stack sfs) \<leadsto>\<^sub>t\<^sub>c\<^sub>o 
         tco_state (TS (v # vs) ((env, []) # sfs))" by simp
+    moreover from evt_lookup have "tco_state (TS vs ((env, [TLookup x]) # sfs)) \<leadsto>\<^sub>t\<^sub>c\<^sub>o
+      TCOS (tco_val v # map tco_val vs) 
+        ((map tco_val env, [], TCOReturn (length env)) # tco_stack sfs)" by simp
     ultimately have "iter (\<leadsto>\<^sub>t\<^sub>c\<^sub>o) (tco_state (TS vs ((env, [TLookup x]) # sfs)))
       (tco_state (TS (v # vs) ((env, []) # sfs)))" by (metis iter_refl iter_step)
     with Nil show ?thesis by simp
@@ -210,11 +215,15 @@ next
   thus ?case 
   proof (cases cd)
     case Nil
-    have "tco_state (TS vs ((env, [TPushCon k]) # sfs)) \<leadsto>\<^sub>t\<^sub>c\<^sub>o
-      TCOS (TCOConst k # map tco_val vs) ((map tco_val env, [], TCOReturn) # tco_stack sfs)" by simp
-    moreover have "TCOS (TCOConst k # map tco_val vs) 
-      ((map tco_val env, [], TCOReturn) # tco_stack sfs) \<leadsto>\<^sub>t\<^sub>c\<^sub>o 
+    have "TCOS (TCOConst k # map tco_val vs) 
+      ((map tco_val env, [], TCOReturn (length env)) # tco_stack sfs) \<leadsto>\<^sub>t\<^sub>c\<^sub>o 
+        TCOS (TCOConst k # map tco_val vs) (tco_stack sfs)" by (metis evtco_return length_map)
+    hence "TCOS (TCOConst k # map tco_val vs) 
+      ((map tco_val env, [], TCOReturn (length env)) # tco_stack sfs) \<leadsto>\<^sub>t\<^sub>c\<^sub>o 
         tco_state (TS (TConst k # vs) ((env, []) # sfs))" by simp
+    moreover have "tco_state (TS vs ((env, [TPushCon k]) # sfs)) \<leadsto>\<^sub>t\<^sub>c\<^sub>o
+      TCOS (TCOConst k # map tco_val vs) 
+        ((map tco_val env, [], TCOReturn (length env)) # tco_stack sfs)" by simp
     ultimately have "iter (\<leadsto>\<^sub>t\<^sub>c\<^sub>o) (tco_state (TS vs ((env, [TPushCon k]) # sfs)))
       (tco_state (TS (TConst k # vs) ((env, []) # sfs)))" by (metis iter_refl iter_step)
     with Nil show ?thesis by simp
@@ -229,27 +238,33 @@ next
   thus ?case 
   proof (cases cd)
     case Nil
-    have "TCOS (map tco_val vs)
-      ((map tco_val env, [TCOPushLam (tco_cd cd') (tco_r cd') (length env)], TCOReturn) # 
-        tco_stack sfs) \<leadsto>\<^sub>t\<^sub>c\<^sub>o  
-          TCOS (TCOLam (map tco_val env) (tco_cd cd') (tco_r cd') # map tco_val vs)
-            ((map tco_val env, [], TCOReturn) # tco_stack sfs)" by (metis evtco_pushlam length_map)
-    hence "tco_state (TS vs ((env, [TPushLam cd' (length env)]) # sfs)) \<leadsto>\<^sub>t\<^sub>c\<^sub>o
-      TCOS (TCOLam (map tco_val env) (tco_cd cd') (tco_r cd') # map tco_val vs) 
-        ((map tco_val env, [], TCOReturn) # tco_stack sfs)" by simp
-    moreover have "TCOS (TCOLam (map tco_val env) (tco_cd cd') (tco_r cd') # map tco_val vs) 
-      ((map tco_val env, [], TCOReturn) # tco_stack sfs) \<leadsto>\<^sub>t\<^sub>c\<^sub>o
+    have "TCOS (map tco_val vs) ((map tco_val env, 
+      [TCOPushLam (tco_cd cd') (tco_r (Suc (length env)) cd') (length env)], 
+        TCOReturn (length env)) # tco_stack sfs) \<leadsto>\<^sub>t\<^sub>c\<^sub>o  TCOS (TCOLam (map tco_val env) (tco_cd cd') 
+          (tco_r (Suc (length env)) cd') # map tco_val vs)
+            ((map tco_val env, [], TCOReturn (length env)) # tco_stack sfs)" 
+      by (metis evtco_pushlam length_map)
+    hence X: "tco_state (TS vs ((env, [TPushLam cd' (length env)]) # sfs)) \<leadsto>\<^sub>t\<^sub>c\<^sub>o
+      TCOS (TCOLam (map tco_val env) (tco_cd cd') (tco_r (Suc (length env)) cd') # map tco_val vs) 
+        ((map tco_val env, [], TCOReturn (length env)) # tco_stack sfs)" by simp
+    have "TCOS (TCOLam (map tco_val env) (tco_cd cd') (tco_r (Suc (length env)) cd') # 
+      map tco_val vs) ((map tco_val env, [], TCOReturn (length env)) # tco_stack sfs) \<leadsto>\<^sub>t\<^sub>c\<^sub>o
+        TCOS (TCOLam (map tco_val env) (tco_cd cd') (tco_r (Suc (length env)) cd') # map tco_val vs) 
+          (tco_stack sfs)" by (metis evtco_return length_map)
+    hence "TCOS (TCOLam (map tco_val env) (tco_cd cd') (tco_r (Suc (length env)) cd') # 
+      map tco_val vs) ((map tco_val env, [], TCOReturn (length env)) # tco_stack sfs) \<leadsto>\<^sub>t\<^sub>c\<^sub>o
         tco_state (TS (TLam env cd' # vs) ((env, []) # sfs))" by simp
-    ultimately have "iter (\<leadsto>\<^sub>t\<^sub>c\<^sub>o) (tco_state (TS vs ((env, [TPushLam cd' (length env)]) # sfs)))
+    with X have "iter (\<leadsto>\<^sub>t\<^sub>c\<^sub>o) (tco_state (TS vs ((env, [TPushLam cd' (length env)]) # sfs)))
       (tco_state (TS (TLam env cd' # vs) ((env, []) # sfs)))" by (metis iter_refl iter_step)
     with Nil show ?thesis by simp
   next
     case (Cons op cd)
     have "TCOS (map tco_val vs) ((map tco_val env, 
-      TCOPushLam (tco_cd cd') (tco_r cd') (length env) # tco_cd (op # cd), tco_r (op # cd)) #
-        tco_stack sfs) \<leadsto>\<^sub>t\<^sub>c\<^sub>o
-          TCOS (TCOLam (map tco_val env) (tco_cd cd') (tco_r cd') # map tco_val vs)
-            ((map tco_val env, tco_cd (op # cd), tco_r (op # cd)) # tco_stack sfs)" 
+      TCOPushLam (tco_cd cd') (tco_r (Suc (length env)) cd') (length env) # tco_cd (op # cd), 
+        tco_r (length env) (op # cd)) # tco_stack sfs) \<leadsto>\<^sub>t\<^sub>c\<^sub>o
+          TCOS (TCOLam (map tco_val env) (tco_cd cd') (tco_r (Suc (length env)) cd') # 
+            map tco_val vs) ((map tco_val env, tco_cd (op # cd), tco_r (length env) (op # cd)) # 
+              tco_stack sfs)" 
       by (metis evtco_pushlam length_map)
     hence 
       "tco_state (TS vs ((env, TPushLam cd' (length env) # op # cd) # sfs)) \<leadsto>\<^sub>t\<^sub>c\<^sub>o
@@ -264,20 +279,34 @@ next
     thus ?thesis
     proof (cases cd')
       case Nil
-      have "TCOS (map tco_val vs) ((tco_val v # map tco_val env', [], TCOReturn) # tco_stack sfs) 
-        \<leadsto>\<^sub>t\<^sub>c\<^sub>o tco_state (TS vs ((v # env', []) # (env, []) # sfs))" by simp
-      hence "iter (\<leadsto>\<^sub>t\<^sub>c\<^sub>o) (TCOS (map tco_val vs) 
-        ((tco_val v # map tco_val env', [], TCOReturn) # tco_stack sfs))
+      have "TCOS (map tco_val vs) ((tco_val v # map tco_val env', [], 
+        TCOReturn (length (tco_val v # map tco_val env'))) # tco_stack sfs) \<leadsto>\<^sub>t\<^sub>c\<^sub>o
+          TCOS (map tco_val vs) (tco_stack sfs)" by (metis evtco_return)
+      hence "TCOS (map tco_val vs) ((tco_val v # map tco_val env', [], 
+        TCOReturn (Suc (length env'))) # tco_stack sfs) \<leadsto>\<^sub>t\<^sub>c\<^sub>o 
+          tco_state (TS vs ((v # env', []) # (env, []) # sfs))" by simp
+      hence X: "iter (\<leadsto>\<^sub>t\<^sub>c\<^sub>o) (TCOS (map tco_val vs) 
+        ((tco_val v # map tco_val env', [], TCOReturn (Suc (length env'))) # tco_stack sfs))
           (tco_state (TS vs ((v # env', []) # (env, []) # sfs)))" by (metis iter_one)
-      moreover have "tco_state (TS (v # TLam env' [] # vs) ((env, [TApply]) # sfs)) \<leadsto>\<^sub>t\<^sub>c\<^sub>o
-        TCOS (map tco_val vs) ((tco_val v # map tco_val env', [], TCOReturn) # tco_stack sfs)" 
-          by simp
-      ultimately have "iter (\<leadsto>\<^sub>t\<^sub>c\<^sub>o) (tco_state (TS (v # TLam env' [] # vs) ((env, [TApply]) # sfs)))
+      have "TCOS (tco_val v # TCOLam (map tco_val env') [] (TCOReturn (Suc (length env'))) # 
+        map tco_val vs) ((map tco_val env, [], TCOJump (length env)) # tco_stack sfs) \<leadsto>\<^sub>t\<^sub>c\<^sub>o
+          TCOS (map tco_val vs) ((tco_val v # map tco_val env', [], TCOReturn (Suc (length env'))) # 
+            tco_stack sfs)" by (metis evtco_jump length_map)
+      hence "tco_state (TS (v # TLam env' [] # vs) ((env, [TApply]) # sfs)) \<leadsto>\<^sub>t\<^sub>c\<^sub>o
+        TCOS (map tco_val vs) ((tco_val v # map tco_val env', [], TCOReturn (Suc (length env'))) # 
+          tco_stack sfs)" by simp
+      with X have "iter (\<leadsto>\<^sub>t\<^sub>c\<^sub>o) (tco_state (TS (v # TLam env' [] # vs) ((env, [TApply]) # sfs)))
         (tco_state (TS vs ((v # env', []) # (env, []) # sfs)))" using iter_step by fast
       with CD Nil show ?thesis by simp
     next
       case (Cons op' cd'')
-      have "tco_state (TS (v # TLam env' (op' # cd'') # vs) ((env, [TApply]) # sfs)) \<leadsto>\<^sub>t\<^sub>c\<^sub>o
+      have "TCOS (tco_val v # TCOLam (map tco_val env') (tco_cd (op' # cd'')) 
+        (tco_r (Suc (length env')) (op' # cd'')) # map tco_val vs) 
+          ((map tco_val env, [], TCOJump (length env)) # tco_stack sfs) \<leadsto>\<^sub>t\<^sub>c\<^sub>o
+            TCOS (map tco_val vs) ((tco_val v # map tco_val env', tco_cd (op' # cd''), 
+              tco_r (Suc (length env')) (op' # cd'')) # tco_stack sfs)" 
+        by (metis evtco_jump length_map)
+      hence "tco_state (TS (v # TLam env' (op' # cd'') # vs) ((env, [TApply]) # sfs)) \<leadsto>\<^sub>t\<^sub>c\<^sub>o
         tco_state (TS vs ((v # env', op' # cd'') # (env, []) # sfs))" by simp
       with Nil Cons show ?thesis by (metis iter_one)
     qed
@@ -286,16 +315,24 @@ next
     thus ?thesis
     proof (cases cd')
       case Nil
-      have "TCOS (map tco_val vs) ((tco_val v # map tco_val env', [], TCOReturn) # 
-        (map tco_val env, tco_cd (op # cd), tco_r (op # cd)) # tco_stack sfs) \<leadsto>\<^sub>t\<^sub>c\<^sub>o
-          tco_state (TS vs ((v # env', []) # (env, op # cd) # sfs))" by simp
-      hence "iter (\<leadsto>\<^sub>t\<^sub>c\<^sub>o) (TCOS (map tco_val vs) ((tco_val v # map tco_val env', [], TCOReturn) # 
-        (map tco_val env, tco_cd (op # cd), tco_r (op # cd)) # tco_stack sfs)) 
-          (tco_state (TS vs ((v # env', []) # (env, op # cd) # sfs)))" by (metis iter_one)
-      moreover have "tco_state (TS (v # TLam env' [] # vs) ((env, TApply # op # cd) # sfs)) \<leadsto>\<^sub>t\<^sub>c\<^sub>o
-        TCOS (map tco_val vs) ((tco_val v # map tco_val env', [], TCOReturn) # 
-          (map tco_val env, tco_cd (op # cd), tco_r (op # cd)) # tco_stack sfs)" by simp
-      ultimately have "iter (\<leadsto>\<^sub>t\<^sub>c\<^sub>o) (tco_state (TS (v # TLam env' [] # vs) 
+      have "TCOS (map tco_val vs) ((tco_val v # map tco_val env', [], 
+        TCOReturn (length (tco_val v # map tco_val env'))) # (map tco_val env, tco_cd (op # cd),
+          tco_r (length env) (op # cd)) # tco_stack sfs) \<leadsto>\<^sub>t\<^sub>c\<^sub>o
+            TCOS (map tco_val vs) ((map tco_val env, tco_cd (op # cd), 
+              tco_r (length env) (op # cd)) # tco_stack sfs)" by (metis evtco_return)
+      hence "TCOS (map tco_val vs) ((tco_val v # map tco_val env', [], 
+        TCOReturn (Suc (length env'))) # (map tco_val env, tco_cd (op # cd), 
+          tco_r (length env) (op # cd)) # tco_stack sfs) \<leadsto>\<^sub>t\<^sub>c\<^sub>o
+            tco_state (TS vs ((v # env', []) # (env, op # cd) # sfs))" by simp
+      hence X: "iter (\<leadsto>\<^sub>t\<^sub>c\<^sub>o) (TCOS (map tco_val vs) ((tco_val v # map tco_val env', [], 
+        TCOReturn (Suc (length env'))) # (map tco_val env, tco_cd (op # cd), 
+          tco_r (length env) (op # cd)) # tco_stack sfs)) 
+            (tco_state (TS vs ((v # env', []) # (env, op # cd) # sfs)))" by (metis iter_one)
+      have "tco_state (TS (v # TLam env' [] # vs) ((env, TApply # op # cd) # sfs)) \<leadsto>\<^sub>t\<^sub>c\<^sub>o
+        TCOS (map tco_val vs) ((tco_val v # map tco_val env', [], TCOReturn (Suc (length env'))) # 
+          (map tco_val env, tco_cd (op # cd), tco_r (length env) (op # cd)) # tco_stack sfs)" 
+            by simp
+      with X have "iter (\<leadsto>\<^sub>t\<^sub>c\<^sub>o) (tco_state (TS (v # TLam env' [] # vs) 
         ((env, TApply # op # cd) # sfs)))
           (tco_state (TS vs ((v # env', []) # (env, op # cd) # sfs)))" 
         using iter_step by fast
