09FlatMemory/FlatMemory.thy
@@ -21,9 +21,9 @@ inductive evalf :: "flat_state \<Rightarrow> flat_state \<Rightarrow> bool" (inf
 | evf_apply [simp]: "cd ! pc = BApply \<Longrightarrow> get_closure h v2 = HLam env' pc' \<Longrightarrow>
     FS h (v1 # v2 # vs) ((Suc pc # env) # sfs) cd \<leadsto>\<^sub>f
       FS h vs ((pc' # v1 # env') # (pc # env) # sfs) cd"
-| evf_return [simp]: "cd ! pc = BReturn \<Longrightarrow> 
+| evf_return [simp]: "cd ! pc = BReturn (length env) \<Longrightarrow> 
     FS h vs ((Suc pc # env) # sfs) cd \<leadsto>\<^sub>f FS h vs sfs cd"
-| evf_jump [simp]: "cd ! pc = BJump \<Longrightarrow> get_closure h v2 = HLam env' pc' \<Longrightarrow>
+| evf_jump [simp]: "cd ! pc = BJump (length env) \<Longrightarrow> get_closure h v2 = HLam env' pc' \<Longrightarrow>
     FS h (v1 # v2 # vs) ((Suc pc # env) # sfs) cd \<leadsto>\<^sub>f FS h vs ((pc' # v1 # env') # sfs) cd"
 
 theorem determinismf: "\<Sigma> \<leadsto>\<^sub>f \<Sigma>' \<Longrightarrow> \<Sigma> \<leadsto>\<^sub>f \<Sigma>'' \<Longrightarrow> \<Sigma>' = \<Sigma>''"
@@ -45,11 +45,11 @@ next
     by (induction "FS h (v1 # v2 # vs) ((Suc pc # env) # sfs) cd" \<Sigma>'' rule: evalf.induct) 
        simp_all 
 next
-  case (evf_return cd pc h vs env sfs)
+  case (evf_return cd pc env h vs sfs)
   from evf_return(2, 1) show ?case 
     by (induction "FS h vs ((Suc pc # env) # sfs) cd" \<Sigma>'' rule: evalf.induct) simp_all 
 next
-  case (evf_jump cd pc h v2 env' pc' v1 vs env sfs)
+  case (evf_jump cd pc env h v2 env' pc' v1 vs sfs)
   from evf_jump(3, 1, 2) show ?case 
     by (induction "FS h (v1 # v2 # vs) ((Suc pc # env) # sfs) cd" \<Sigma>'' rule: evalf.induct) 
        simp_all 
